Refactor extended ghost map for more features

theories/interop/extra_ghost_state/persistent_ghost_map.v
@@ -11,24 +11,58 @@ From melocoton.interop.extra_ghost_state Require Import gmap_view_pluspers.
 (** The CMRA we need.
 FIXME: This is intentionally discrete-only, but
 should we support setoids via [Equiv]? *)
-Class pgmG `{SI: indexT} Σ (K V Vpers : Type) (Fpers : V → Vpers) `{Countable K} := GhostMapG {
-  pgm_inG : inG Σ (gmap_view_plusR K (leibnizO V) (leibnizO Vpers) Fpers);
+Class PGMData : Type := {
+  K : Type;
+  V : Type;
+  Vpers : Type;
+  Fpers : V → Vpers;
+  HEq :> EqDecision K;
+  HCount :> Countable K;
+  Pmap : gmap K V → Prop;
+  Pmap_mono (m1 m2 : gmap K V) : Pmap m1 → m2 ⊆ m1 → Pmap m2;
+  Pmap_init : Pmap ∅
+}.
+
+Global Program Instance EGV_PGM `{SI: indexT} `{D : PGMData} : ExtendedGmapView := {|
+  gmap_view_pluspers.K := K;
+  gmap_view_pluspers.V := leibnizO V;
+  gmap_view_pluspers.Vpers := leibnizO Vpers;
+  gmap_view_pluspers.Fpers := Fpers;
+  gmap_view_pluspers.Pmap n := Pmap;
+|}.
+Next Obligation.
+Proof.
+  intros SI D n1 n2 m1 m2 H1 _ Helem; cbn.
+  eapply Pmap_mono; first exact H1.
+  eapply map_subseteq_spec.
+  intros k v Hin.
+  specialize (Helem k v Hin); inversion Helem; simplify_eq.
+  cbv in H2. simplify_eq. done.
+Defined.
+Next Obligation. intros ???; exists ∅; apply Pmap_init. Defined.
+
+Global Instance EGV_Discrete `{SI: indexT} `{D : PGMData} : PmapDiscrete (EGV_PGM).
+Proof. by intros m n Hm. Qed.
+
+
+Class pgmG `{SI: indexT} Σ (D : PGMData) := GhostMapG {
+  pgm_inG : inG Σ (gmap_view_plusR _);
 }.
 Local Existing Instance pgm_inG.
 
-Definition pgmΣ `{SI: indexT} (K V Vpers : Type) (Fpers : V → Vpers) `{Countable K} : gFunctors :=
-  #[ GFunctor (gmap_view_plusR K (leibnizO V) (leibnizO Vpers) Fpers) ].
+Definition pgmΣ `{SI: indexT} (D' : PGMData) : gFunctors :=
+  #[ GFunctor (gmap_view_plusR _) ].
 
-Global Instance subG_pgmΣ `{SI: indexT} Σ (K V Vpers : Type) (Fpers : V → Vpers) `{Countable K} :
-  subG (pgmΣ K V Vpers Fpers) Σ → pgmG Σ K V Vpers Fpers.
+Global Instance subG_pgmΣ `{SI: indexT} Σ (D : PGMData) :
+  subG (pgmΣ D) Σ → pgmG Σ D.
 Proof. solve_inG. Qed.
 
 Section definitions.
-  Context `{pgmG Σ K V Vpers Fpers}.
+  Context `{pgmG Σ}.
 
   Local Definition pgm_auth_def
       (γ : gname) (q : Qp) (m : gmap K V) : iProp Σ :=
-    own γ (gmap_view_plus_auth (V:=leibnizO V) (Vpers := leibnizO Vpers) (Fpers := Fpers) (DfracOwn q) m).
+    own γ (gmap_view_plus_auth (DfracOwn q) m).
   Local Definition pgm_auth_aux : seal (@pgm_auth_def).
   Proof. by eexists. Qed.
   Definition pgm_auth := pgm_auth_aux.(unseal).
@@ -37,7 +71,7 @@ Section definitions.
 
   Local Definition pgm_elem_def
       (γ : gname) (k : K) (dq : dfrac) (v : V) : iProp Σ :=
-    own γ (gmap_view_plus_frag (V:=leibnizO V) (Vpers := leibnizO Vpers) (Fpers := Fpers) k dq v).
+    own γ (gmap_view_plus_frag k dq v).
   Local Definition pgm_elem_aux : seal (@pgm_elem_def).
   Proof. by eexists. Qed.
   Definition pgm_elem := pgm_elem_aux.(unseal).
@@ -46,7 +80,7 @@ Section definitions.
 
   Local Definition pgm_pers_def
       (γ : gname) (k : K) (vp : Vpers) : iProp Σ :=
-    own γ (gmap_view_plus_pers (V:=leibnizO V) (Vpers := leibnizO Vpers) (Fpers := Fpers) k vp).
+    own γ (gmap_view_plus_pers k vp).
   Local Definition pgm_pers_aux : seal (@pgm_pers_def).
   Proof. by eexists. Qed.
   Definition pgm_pers := pgm_pers_aux.(unseal).
@@ -73,7 +107,7 @@ Local Ltac unseal := rewrite
   ?pgm_pers_unseal /pgm_pers_def.
 
 Section lemmas.
-  Context `{pgmG Σ K V Vpers Fpers}.
+  Context `{pgmG Σ}.
   Implicit Types (k : K) (v : V) (dq : dfrac) (q : Qp) (m : gmap K V) (vp : Vpers).
 
   (** * Lemmas about the map elements *)
@@ -94,7 +128,7 @@ Section lemmas.
 
   Local Lemma pgm_elems_unseal γ m dq :
     ([∗ map] k ↦ v ∈ m, k □↪[γ]{dq} v) ==∗
-    own γ ([^op map] k↦v ∈ m, gmap_view_plus_frag (V:=leibnizO V) k dq v).
+    own γ ([^op map] k↦v ∈ m, gmap_view_plus_frag k dq v).
   Proof.
     unseal. destruct (decide (m = ∅)) as [->|Hne].
     - rewrite !big_opM_empty. iIntros "_". iApply own_unit.
@@ -103,7 +137,7 @@ Section lemmas.
 
   Local Lemma pgm_perms_unseal γ (mpers : gmap K Vpers) dq :
     ([∗ map] k ↦ vp ∈ mpers, k □↪[γ]= vp) ==∗
-    own γ ([^op map] k↦vp ∈ mpers, gmap_view_plus_pers (V:=leibnizO V) (Vpers:=leibnizO Vpers) k vp).
+    own γ ([^op map] k↦vp ∈ mpers, gmap_view_plus_pers k vp).
   Proof.
     unseal. destruct (decide (mpers = ∅)) as [->|Hne].
     - rewrite !big_opM_empty. iIntros "_". iApply own_unit.
@@ -113,14 +147,14 @@ Section lemmas.
   Lemma pgm_elem_valid k γ dq v : k □↪[γ]{dq} v -∗ ⌜✓ dq⌝.
   Proof.
     unseal. iIntros "Helem".
-    iDestruct (own_valid with "Helem") as %?%gmap_view_plus_frag_valid.
+    iDestruct (own_valid with "Helem") as %(?&?)%gmap_view_plus_frag_valid.
     done.
   Qed.
   Lemma pgm_elem_valid_2 k γ dq1 dq2 v1 v2 :
     k □↪[γ]{dq1} v1 -∗ k □↪[γ]{dq2} v2 -∗ ⌜✓ (dq1 ⋅ dq2) ∧ v1 = v2⌝.
   Proof.
     unseal. iIntros "H1 H2".
-    iDestruct (own_valid_2 with "H1 H2") as %?%gmap_view_plus_frag_op_valid_L.
+    iDestruct (own_valid_2 with "H1 H2") as %(?&?&?)%gmap_view_plus_frag_op_valid_L.
     done.
   Qed.
   Lemma pgm_elem_agree k γ dq1 dq2 v1 v2 :
@@ -134,15 +168,15 @@ Section lemmas.
     k □↪[γ]{dq1} v1 -∗ k □↪[γ]= vp2 -∗ ⌜Fpers v1 = vp2⌝.
   Proof.
     unseal. iIntros "Helem1 Helem2".
-    iDestruct (own_valid_2 with "Helem1 Helem2") as %?%gmap_view_plus_frag_pers_op_valid_L.
-    iPureIntro; apply H1.
+    iDestruct (own_valid_2 with "Helem1 Helem2") as %(?&?&?)%gmap_view_plus_frag_pers_op_valid_L.
+    iPureIntro; done.
   Qed.
   Lemma pgm_pers_agree k γ vp1 vp2 :
     k □↪[γ]= vp1 -∗ k □↪[γ]= vp2 -∗ ⌜vp1 = vp2⌝.
   Proof.
     unseal. iIntros "Helem1 Helem2".
-    iDestruct (own_valid_2 with "Helem1 Helem2") as %?%gmap_view_plus_pers_op_valid_L.
-    iPureIntro; apply H1.
+    iDestruct (own_valid_2 with "Helem1 Helem2") as %(?&Hn)%gmap_view_plus_pers_op_valid_L.
+    iPureIntro; done.
   Qed.
 
   (** Get the persistent part. *)
@@ -187,18 +221,20 @@ Section lemmas.
 
   (** * Lemmas about [pgm_auth] *)
   Lemma pgm_alloc_strong P m :
+    Pmap m →
     pred_infinite P →
     ⊢ |==> ∃ γ, ⌜P γ⌝ ∗ pgm_auth γ 1 m ∗ [∗ map] k ↦ v ∈ m, k □↪[γ] v.
   Proof.
     unseal. intros.
-    iMod (own_alloc_strong (gmap_view_plus_auth (V:=leibnizO V) (DfracOwn 1) ∅) P)
+    iMod (own_alloc_strong (gmap_view_plus_auth (DfracOwn 1) ∅) P)
       as (γ) "[% Hauth]"; first done.
-    { apply gmap_view_plus_auth_valid. }
+    { apply gmap_view_plus_auth_valid. intros ?. apply Pmap_init. }
     iExists γ. iSplitR; first done.
     rewrite -big_opM_own_1 -own_op. iApply (own_update with "Hauth").
-    etrans; first apply: (gmap_view_plus_alloc_big (V:=leibnizO V) _ m (DfracOwn 1)).
+    etrans; first eapply (gmap_view_plus_alloc_big EGV_PGM ∅ m (DfracOwn 1)).
     - apply map_disjoint_empty_r.
     - done.
+    - intros ??. by rewrite map_union_empty.
     - rewrite right_id -big_opM_op.
       setoid_rewrite <- gmap_view_plus_frag_get_persistent.
       done.
@@ -208,11 +244,15 @@ Section lemmas.
     ⊢ |==> ∃ γ, ⌜P γ⌝ ∗ pgm_auth γ 1 (∅ : gmap K V).
   Proof.
     intros. iMod (pgm_alloc_strong P ∅) as (γ) "(% & Hauth & _)"; eauto.
+    apply Pmap_init.
   Qed.
   Lemma pgm_alloc m :
+    Pmap m →
     ⊢ |==> ∃ γ, pgm_auth γ 1 m ∗ [∗ map] k ↦ v ∈ m, k □↪[γ] v.
   Proof.
+    intros HPmap.
     iMod (pgm_alloc_strong (λ _, True) m) as (γ) "[_ Hmap]".
+    - done.
     - by apply pred_infinite_True.
     - eauto.
   Qed.
@@ -220,6 +260,7 @@ Section lemmas.
     ⊢ |==> ∃ γ, pgm_auth γ 1 (∅ : gmap K V).
   Proof.
     intros. iMod (pgm_alloc ∅) as (γ) "(Hauth & _)"; eauto.
+    eapply Pmap_init.
   Qed.
 
   Global Instance pgm_auth_timeless γ q m : Timeless (pgm_auth γ q m).
@@ -230,17 +271,23 @@ Section lemmas.
     AsFractional (pgm_auth γ q m) (λ q, pgm_auth γ q m)%I q.
   Proof. split; first done. apply _. Qed.
 
+  Lemma pgm_auth_valid_prop γ q m : pgm_auth γ q m -∗ ⌜Pmap m⌝%Qp.
+  Proof.
+    unseal. iIntros "Hauth".
+    iDestruct (own_valid with "Hauth") as %(?&?)%gmap_view_plus_auth_dfrac_valid.
+    iPureIntro. apply (H1 zero).
+  Qed.
   Lemma pgm_auth_valid γ q m : pgm_auth γ q m -∗ ⌜q ≤ 1⌝%Qp.
   Proof.
     unseal. iIntros "Hauth".
-    iDestruct (own_valid with "Hauth") as %?%gmap_view_plus_auth_dfrac_valid.
+    iDestruct (own_valid with "Hauth") as %(?&?)%gmap_view_plus_auth_dfrac_valid.
     done.
   Qed.
   Lemma pgm_auth_valid_2 γ q1 q2 m1 m2 :
     pgm_auth γ q1 m1 -∗ pgm_auth γ q2 m2 -∗ ⌜(q1 + q2 ≤ 1)%Qp ∧ m1 = m2⌝.
   Proof.
     unseal. iIntros "H1 H2".
-    iDestruct (own_valid_2 with "H1 H2") as %[??]%gmap_view_plus_auth_dfrac_op_valid_L.
+    iDestruct (own_valid_2 with "H1 H2") as %(?&?&?)%gmap_view_plus_auth_dfrac_op_valid_L.
     done.
   Qed.
   Lemma pgm_auth_agree γ q1 q2 m1 m2 :
@@ -256,7 +303,7 @@ Section lemmas.
     pgm_auth γ q m -∗ k □↪[γ]{dq} v -∗ ⌜m !! k = Some v⌝.
   Proof.
     unseal. iIntros "Hauth Hel".
-    iDestruct (own_valid_2 with "Hauth Hel") as %[?[??]]%gmap_view_plus_both_dfrac_valid_L.
+    iDestruct (own_valid_2 with "Hauth Hel") as %[?[?(?&?)]]%gmap_view_plus_both_dfrac_valid_L.
     eauto.
   Qed.
 
@@ -266,7 +313,7 @@ Section lemmas.
     unseal. iIntros "Hauth Hel".
     iDestruct (own_valid_2 with "Hauth Hel") as %HH.
     unshelve eapply cmra_valid_validN in HH. 1: exact zero.
-    eapply gmap_view_plus_pers_both_dfrac_validN in HH as (Hq&v&Hv1&Hv2).
+    eapply gmap_view_plus_pers_both_dfrac_validN in HH as (Hq&v&Hv1&Hv2&Hprop).
     apply discrete in Hv1,Hv2. 2-3: apply _.
     apply leibniz_equiv in Hv1,Hv2.
     iPureIntro. by eexists.
@@ -274,27 +321,31 @@ Section lemmas.
 
   Lemma pgm_insert {γ m} k v :
     m !! k = None →
+    (Pmap m → Pmap (<[k := v]> m)) →
     pgm_auth γ 1 m ==∗ pgm_auth γ 1 (<[k := v]> m) ∗ k □↪[γ] v.
   Proof.
-    unseal. intros ?. rewrite -own_op.
+    unseal. intros ??. rewrite -own_op.
     iApply own_update. rewrite gmap_view_plus_frag_get_persistent. 
     apply: gmap_view_plus_alloc; done.
   Qed.
   Lemma pgm_insert_persist {γ m} k v :
     m !! k = None →
+    (Pmap m → Pmap (<[k := v]> m)) →
     pgm_auth γ 1 m ==∗ pgm_auth γ 1 (<[k := v]> m) ∗ k □↪[γ]□ v.
   Proof.
-    iIntros (?) "Hauth".
-    iMod (pgm_insert k with "Hauth") as "[$ Helem]"; first done.
+    iIntros (??) "Hauth".
+    iMod (pgm_insert k with "Hauth") as "[$ Helem]"; try done.
     iApply pgm_elem_persist. done.
   Qed.
 
   Lemma pgm_update {γ m k v} w :
     Fpers v = Fpers w →
+    (Pmap m → Pmap (<[k := w]> m)) →
     pgm_auth γ 1 m -∗ k □↪[γ] v ==∗ pgm_auth γ 1 (<[k := w]> m) ∗ k □↪[γ] w.
   Proof.
-    unseal. intros Hpers. apply bi.wand_intro_r. rewrite -!own_op.
-    apply own_update. apply: gmap_view_plus_update. done.
+    unseal. intros Hpers Hprop. apply bi.wand_intro_r. rewrite -!own_op.
+    apply own_update. apply: gmap_view_plus_update; first done.
+    intros n; apply Hprop.
   Qed.
 
   (** Big-op versions of above lemmas *)
@@ -311,10 +362,11 @@ Section lemmas.
 
   Lemma pgm_insert_big {γ m} m' :
     m' ##ₘ m →
+    (Pmap m → Pmap (m' ∪ m)) →
     pgm_auth γ 1 m ==∗
     pgm_auth γ 1 (m' ∪ m) ∗ ([∗ map] k ↦ v ∈ m', k □↪[γ] v).
   Proof.
-    unseal. intros ?. rewrite -big_opM_own_1 -own_op.
+    unseal. intros ??. rewrite -big_opM_own_1 -own_op.
     apply own_update. setoid_rewrite gmap_view_plus_frag_get_persistent.
     rewrite big_opM_op.
     apply: gmap_view_plus_alloc_big; done.
@@ -322,37 +374,83 @@ Section lemmas.
 
   Lemma pgm_insert_persist_big {γ m} m' :
     m' ##ₘ m →
+    (Pmap m → Pmap (m' ∪ m)) →
     pgm_auth γ 1 m ==∗
     pgm_auth γ 1 (m' ∪ m) ∗ ([∗ map] k ↦ v ∈ m', k □↪[γ]□ v).
   Proof.
-    iIntros (Hdisj) "Hauth".
-    iMod (pgm_insert_big m' with "Hauth") as "[$ Helem]"; first done.
+    iIntros (Hdisj Hprop) "Hauth".
+    iMod (pgm_insert_big m' with "Hauth") as "[$ Helem]"; try done.
     iApply big_sepM_bupd. iApply (big_sepM_impl with "Helem").
     iIntros "!#" (k v) "_". iApply pgm_elem_persist.
   Qed.
-(*
-  Lemma pgm_delete_big {γ m} m0 :
-    pgm_auth γ 1 m -∗
-    ([∗ map] k↦v ∈ m0, k □↪[γ] v) ==∗
-    pgm_auth γ 1 (m ∖ m0).
-  Proof.
-    iIntros "Hauth Hfrag". iMod (pgm_elems_unseal with "Hfrag") as "Hfrag".
-    unseal. iApply (own_update_2 with "Hauth Hfrag").
-    apply: gmap_view_plus_delete_big.
-  Qed. *)
 
   Theorem pgm_update_big {γ m} m0 m1 :
     dom m0 = dom m1 →
     (∀ k v0 v1, m0 !! k = Some v0 → m1 !! k = Some v1 → Fpers v0 = Fpers v1) →
+    (Pmap (m1 ∪ m)) →
     pgm_auth γ 1 m -∗
     ([∗ map] k↦v ∈ m0, k □↪[γ] v) ==∗
     pgm_auth γ 1 (m1 ∪ m) ∗
         [∗ map] k↦v ∈ m1, k □↪[γ] v.
   Proof.
-    iIntros (??) "Hauth Hfrag". iMod (pgm_elems_unseal with "Hfrag") as "Hfrag".
+    iIntros (???) "Hauth Hfrag". iMod (pgm_elems_unseal with "Hfrag") as "Hfrag".
     unseal. rewrite -big_opM_own_1 -own_op.
     iApply (own_update_2 with "Hauth Hfrag").
     apply: gmap_view_plus_update_big; done.
+  Qed.
+
+  Lemma pgm_lookup_prop {γ q m} m0 :
+    ([∗ map] k↦v ∈ m0, ∃ dq, k □↪[γ]{dq} v) -∗
+    ⌜Pmap m0⌝.
+  Proof.
+    iIntros "Hfrag". unseal.
+    epose (∃ (m1 : gmap K (prod V dfrac)), ⌜dom m1 = dom m0⌝ ∧ ⌜∀ k v dq, m1 !! k = Some (v,dq) → m0 !! k = Some v⌝ ∧ (⌜m1 = ∅⌝ ∨ own γ (◯V (fmap (λ '(v,dq), (Some (dq, to_agree v), to_agree (Fpers v))) m1)
+            : gmap_view_pluspers.gmap_view_plusUR _)))%I.
+    iAssert b with "[Hfrag]" as "(%m1&%Hdom&%Hcont&[->|Hm1])"; unfold b; clear b.
+    - iStopProof.
+      induction m0 as [|k v m0 Hne IH] using map_ind; iStartProof; iIntros "Hfrag".
+      { iExists ∅; iSplit. 1: rewrite !dom_empty_L //.
+        iSplit; last by iLeft.
+        iPureIntro. intros k v ? []%lookup_empty_Some. }
+      iPoseProof (big_sepM_insert with "Hfrag") as "((%dq&Hpto)&Hfrag)"; first done.
+      iPoseProof (IH with "Hfrag") as "(%m1&%Hdom&%Hcont&[->|IH])".
+      + iExists {[ k := (v,dq) ]}. iSplit.
+        1: iPureIntro; rewrite dom_empty_L in Hdom; rewrite dom_insert_L dom_singleton_L -Hdom; set_solver.
+        iSplit; last (iRight; erewrite map_fmap_singleton; iApply "Hpto").
+        iPureIntro. intros k' v' dq' [<- [= <- <-]]%lookup_singleton_Some. by rewrite lookup_insert.
+      + iExists (<[ k := (v,dq) ]> m1). iSplit.
+        1: iPureIntro; rewrite dom_insert_L; set_solver.
+        iSplit.
+        { iPureIntro; intros k' v' dq' [[-> [= -> ->]]|[Hne1 HH]]%lookup_insert_Some.
+          1: by rewrite lookup_insert.
+          rewrite lookup_insert_ne; first by eapply Hcont. done. }
+        iRight.
+        iPoseProof (own_op with "[$Hpto $IH]") as "HH".
+        unfold gmap_view_plus_frag. rewrite -view_frag_op.
+        rewrite fmap_insert.
+        rewrite (@insert_singleton_op _ _ _ _ ((prodR (optionR (prodR dfracR (agreeR (leibnizO V)))) (agreeR (leibnizO Vpers))))).
+        2: { rewrite lookup_fmap. destruct (m1 !! k) eqn:Heqn; last done.
+             eapply elem_of_dom_2 in Heqn. eapply not_elem_of_dom in Hne. by rewrite Hdom in Heqn. }
+        done.
+    - iPureIntro. enough (m0 = ∅) as -> by eapply Pmap_init.
+      rewrite dom_empty_L in Hdom. eapply dom_empty_inv_L. done.
+    - iDestruct (own_valid with "Hm1") as %Hm1.
+      iPureIntro.
+      apply view_frag_valid in Hm1.
+      specialize (Hm1 zero) as (mv&Hmv&Hmprop).
+      cbn in *.
+      eapply Pmap_mono; first done.
+      eapply map_subseteq_spec.
+      intros k v Hin.
+      destruct (m1 !! k) as [[v' dq]|] eqn:Heq; last first.
+      { exfalso. apply elem_of_dom_2 in Hin. eapply not_elem_of_dom in Heq. by rewrite Hdom in Heq. }
+      epose proof (Hcont _ _ _ Heq) as Heq2. simplify_eq.
+      eapply (map_Forall_lookup_1 _ _ k) in Hmv; last first.
+      { rewrite lookup_fmap Heq; done. }
+      destruct Hmv as (v'&Hmv'&Hagr1&Hagr2&Hdv). cbn in *.
+      rewrite Hmv'. f_equal.
+      eapply @to_agree_injN, discrete_iff in Hagr2; last apply _.
+      done.
   Qed.
 
 End lemmas.
